Finish bvl_inline implementation and proofs
The implementation works by walking the code table from top
to bottom. The loop inlines to-be-inlined functions and then
checks whether the resulting code is small enough (and not
recursive) to decide whether it should put the function's
body into the map of to-be-inlined functions.

The proof is interesting because it uses a semantic relation
rather than the usual syntactic approach.

Progress on #51

Thw issue will be closed when the magic number in bvl_to_bvi
has been made into compiler configuration. Currently a
function is small if its size is less than 3. (This
optimisation is turned off by setting the limit to 0.)

compiler/backend/bvl_inlineScript.sml
@@ -34,6 +34,80 @@ val inline_def = tDefine "inline" `
 
 val inline_ind = theorem"inline_ind";
 
+(* This definition is written to exit as soon as possible. *)
+val is_small_aux_def = tDefine "is_small_aux" `
+  (is_small_aux n [] = n) /\
+  (is_small_aux n (x::y::xs) =
+     if n = 0 then n else
+       let n = is_small_aux n [x] in if n = 0 then n else
+         is_small_aux n (y::xs)) /\
+  (is_small_aux n [Var v] = n) /\
+  (is_small_aux n [If x1 x2 x3] =
+     let n = n - 1 in if n = 0 then 0 else
+     let n = is_small_aux n [x1] in if n = 0 then 0 else
+     let n = is_small_aux n [x2] in if n = 0 then 0 else
+       is_small_aux n [x3]) /\
+  (is_small_aux n [Let xs x2] =
+     let n = n - 1 in if n = 0 then 0 else
+     let n = is_small_aux n xs in if n = 0 then 0 else
+       is_small_aux n [x2]) /\
+  (is_small_aux n [Raise x1] =
+     let n = n - 1 in if n = 0 then 0 else
+       is_small_aux n [x1]) /\
+  (is_small_aux n [Handle x1 x2] =
+     let n = n - 1 in if n = 0 then 0 else
+     let n = is_small_aux n [x1] in if n = 0 then 0 else
+       is_small_aux n [x2]) /\
+  (is_small_aux n [Op op xs] =
+     let n = n - 1 in if n = 0 then 0 else
+       is_small_aux n xs) /\
+  (is_small_aux n [Tick x] = is_small_aux n [x]) /\
+  (is_small_aux n [Call ticks dest xs] =
+     let n = n - 1 in if n = 0 then 0 else
+       is_small_aux n xs)`
+  (WF_REL_TAC `measure (exp1_size o SND)`);
+
+val is_small_def = Define `
+  is_small limit e = ~(is_small_aux limit [e] = 0)`;
+
+val is_rec_def = tDefine "is_rec" `
+  (is_rec n [] = F) /\
+  (is_rec n (x::y::xs) =
+     if is_rec n [x] then T else
+       is_rec n (y::xs)) /\
+  (is_rec n [Var v] = F) /\
+  (is_rec n [If x1 x2 x3] =
+     if is_rec n [x1] then T else
+     if is_rec n [x2] then T else
+       is_rec n [x3]) /\
+  (is_rec n [Let xs x2] =
+     if is_rec n xs then T else
+       is_rec n [x2]) /\
+  (is_rec n [Raise x1] = is_rec n [x1]) /\
+  (is_rec n [Handle x1 x2] =
+     if is_rec n [x1] then T else
+       is_rec n [x2]) /\
+  (is_rec n [Op op xs] = is_rec n xs) /\
+  (is_rec n [Tick x] = is_rec n [x]) /\
+  (is_rec n [Call ticks dest xs] =
+     if dest = SOME n then T else is_rec n xs)`
+  (WF_REL_TAC `measure (exp1_size o SND)`);
+
+val must_inline_def = Define `
+  must_inline name limit e =
+    if is_small limit e then ~(is_rec name [e]) else F`
+
+val inline_all_def = Define `
+  (inline_all limit cs [] aux = REVERSE aux) /\
+  (inline_all limit cs ((n,arity,e1)::xs) aux =
+     let e2 = HD (inline cs [e1]) in
+     let cs2 = if must_inline n limit e2 then insert n (arity,e2) cs else cs in
+       inline_all limit cs2 xs ((n,arity,e2)::aux))`;
+
+val compile_prog_def = Define `
+  compile_prog limit prog =
+    if limit = 0 then prog else inline_all limit LN prog []`
+
 val LENGTH_inline = store_thm("LENGTH_inline",
   ``!cs xs. LENGTH (inline cs xs) = LENGTH xs``,
   recInduct inline_ind \\ REPEAT STRIP_TAC
